src/lowparse/LowParse.Spec.ConstInt32.fst
@@ -1,6 +1,6 @@
 module LowParse.Spec.ConstInt32
 
-(* LowParse specification module for parsing 32 bits = 4 bytes constants
+(* LowParse specification module for parsing 32 bits = 4 bytes unsigned constants
 
    Examples:
 
@@ -9,11 +9,13 @@ module LowParse.Spec.ConstInt32
 
 *)
 
+(* TODO: support big endian constants *)
+
 include FStar.Endianness
 
 include LowParse.Spec.Base
 include LowParse.Spec.Combinators
-include LowParse.Spec.BoundedInt
+include LowParse.Spec.Int32le
 
 module U32 = FStar.UInt32
 module U8 = FStar.UInt8
@@ -30,115 +32,26 @@ let parse_constint32le_kind
 : parser_kind
 = strong_parser_kind 4 4 None
 
-let decode_int32_le
-  (b: bytes { Seq.length b == 4 } )
-: Tot (v: U32.t { 0 <= U32.v v /\ U32.v v < 4294967296 } )
-= lemma_le_to_n_is_bounded b;
-  M.pow2_le_compat 32 32;
-  let res = le_to_n b in
-  assert (0 <= res /\ res < 4294967296);
-  U32.uint_to_t res
-
-let decode_int32_le_injective
-  (b1 : bytes { Seq.length b1 == 4 } )
-  (b2 : bytes { Seq.length b2 == 4 } )
-: Lemma (decode_int32_le b1 == decode_int32_le b2
-        ==>
-        b1 == b2)
-= if (decode_int32_le b1) = (decode_int32_le b2) then
-  begin
-    lemma_le_to_n_is_bounded b1;
-    lemma_le_to_n_is_bounded b2;
-    assert (U32.v (U32.uint_to_t (le_to_n b1)) == le_to_n b1);
-    assert (U32.v (U32.uint_to_t (le_to_n b2)) == le_to_n b2);
-    assert (le_to_n b1 == le_to_n b2);
-    le_to_n_inj b1 b2
-  end
-  else
-    ()
-
-let decode_int32_le_total_constant () : Lemma (make_total_constant_size_parser_precond 4 U32.t decode_int32_le)
-= Classical.forall_intro_2 decode_int32_le_injective
-
-let parse_int32_le () : Tot (parser (total_constant_size_parser_kind 4) U32.t)
-= decode_int32_le_total_constant () ;
-  make_total_constant_size_parser 4 U32.t decode_int32_le
-
-let le_to_n_0_eq
-  (b : bytes { Seq.length b == 0 } )
-: Lemma (le_to_n b == 0)
-= reveal_le_to_n b
-
-let le_to_n_1_eq
-  (b : bytes { Seq.length b == 1 } )
-: Lemma (le_to_n b == 
-    U8.v (Seq.index b 0))
-= assert_norm (pow2 8 == 256);
-  reveal_le_to_n b;
-  le_to_n_0_eq (Seq.tail b)
-
-let le_to_n_2_eq
-  (b : bytes { Seq.length b == 2 } )
-: Lemma (le_to_n b == 
-    U8.v (Seq.index b 0) + 
-    256 `FStar.Mul.op_Star` (U8.v (Seq.index b 1)))
-= assert_norm (pow2 8 == 256);
-  reveal_le_to_n b;
-  le_to_n_1_eq (Seq.tail b)
-
-let le_to_n_3_eq
-  (b : bytes { Seq.length b == 3 } )
-: Lemma (le_to_n b == 
-    U8.v (Seq.index b 0) + 
-    256 `FStar.Mul.op_Star` (U8.v (Seq.index b 1) + 
-    256 `FStar.Mul.op_Star` (U8.v (Seq.index b 2))))
-= assert_norm (pow2 8 == 256);
-  reveal_le_to_n b;
-  le_to_n_2_eq (Seq.tail b)
-
-let le_to_n_4_eq
-  (b : bytes { Seq.length b == 4 } )
-: Lemma (le_to_n b == 
-    U8.v (Seq.index b 0) + 
-    256 `FStar.Mul.op_Star` (U8.v (Seq.index b 1) + 
-    256 `FStar.Mul.op_Star` (U8.v (Seq.index b 2) + 
-    256 `FStar.Mul.op_Star` (U8.v (Seq.index b 3)))))
-= assert_norm (pow2 8 == 256);
-  reveal_le_to_n b;
-  le_to_n_3_eq (Seq.tail b)
-
-let decode_int32_le_eq
-  (b : bytes { Seq.length b == 4 } )
-: Lemma
-  (U32.v (decode_int32_le b) ==
-    U8.v (Seq.index b 0) + 
-    256 `FStar.Mul.op_Star` (U8.v (Seq.index b 1) + 
-    256 `FStar.Mul.op_Star` (U8.v (Seq.index b 2) + 
-    256 `FStar.Mul.op_Star` (U8.v (Seq.index b 3)))))
-= lemma_le_to_n_is_bounded b;
-  assert (U32.v (decode_int32_le b) == le_to_n b);
-  le_to_n_4_eq b
-
-let decode_constint32_le
+let decode_constint32le
   (v: nat {0 <= v /\ v < 4294967296 } )
   (b: bytes { Seq.length b == 4 } )
 : Tot (option (constint32 v))
-= let v' = decode_int32_le b in
+= let v' = decode_int32le b in
     if U32.v v' = v then
       Some v'
     else
       None
 
-let decode_constint32_le_injective'
+let decode_constint32le_injective'
   (v: nat { 0 <= v /\ v < 4294967296 } )
   (b1: bytes { Seq.length b1 == 4 } )
   (b2: bytes { Seq.length b2 == 4 } )
 : Lemma
-  ((Some? (decode_constint32_le v b1) \/ Some? (decode_constint32_le v b2))
-   /\ (decode_constint32_le v b1 == decode_constint32_le v b2) 
+  ((Some? (decode_constint32le v b1) \/ Some? (decode_constint32le v b2))
+   /\ (decode_constint32le v b1 == decode_constint32le v b2) 
    ==> Seq.equal b1 b2)
-= let res1 = decode_constint32_le v b1 in
-  let res2 = decode_constint32_le v b2 in
+= let res1 = decode_constint32le v b1 in
+  let res2 = decode_constint32le v b2 in
   match res1 with
   | Some v1 ->
     assert ( U32.v v1 == v );
@@ -146,28 +59,28 @@ let decode_constint32_le_injective'
     | Some v2 ->
       assert ( U32.v v2 == v );
       assert ( v1 == v2 );
-      decode_int32_le_injective b1 b2
+      decode_int32le_injective b1 b2
     | None -> ())
   | None -> ()
 
-let decode_constint32_le_injective
+let decode_constint32le_injective
   (v: nat { 0 <= v /\ v < 4294967296 } )
 : Lemma
-  (make_constant_size_parser_precond 4 (constint32 v) (decode_constint32_le v))
-= Classical.forall_intro_2 (decode_constint32_le_injective' v)
+  (make_constant_size_parser_precond 4 (constint32 v) (decode_constint32le v))
+= Classical.forall_intro_2 (decode_constint32le_injective' v)
 
 let parse_constint32le
   (v: nat { 0 <= v /\ v < 4294967296 } )
 : Tot (parser parse_constint32le_kind (constint32 v))
-= decode_constint32_le_injective v;
-  make_constant_size_parser 4 (constint32 v) (decode_constint32_le v)
+= decode_constint32le_injective v;
+  make_constant_size_parser 4 (constint32 v) (decode_constint32le v)
 
 let parse_constint32le_unfold
   (v: nat { 0 <= v /\ v < 4294967296 } )
   (input: bytes)
 : Lemma 
   (parse (parse_constint32le v) input ==
-  (let res = parse (parse_int32_le ()) input in
+  (let res = parse parse_int32le input in
      match res with
      | Some (x, consumed) ->
        if U32.v x = v && consumed = 4 then
@@ -175,7 +88,7 @@ let parse_constint32le_unfold
        else
          None
      | None -> None))
-= let res = parse (parse_int32_le ()) input in
+= let res = parse parse_int32le input in
     match res with
     | Some (x, consumed) ->
       if U32.v x = v && consumed = 4 then
