src/lowparse/LowParse.Spec.Int32le.fst
@@ -1,0 +1,114 @@
+module LowParse.Spec.Int32le
+
+(* LowParse specification module for parsing unconstrainted 32 bits = 4 bytes unsigned little endian integers
+
+   Examples:
+
+   uint32le foo
+
+*)
+
+include FStar.Endianness
+
+include LowParse.Spec.Base
+include LowParse.Spec.Combinators
+
+module U32 = FStar.UInt32
+module U8 = FStar.UInt8
+module Seq = FStar.Seq
+module M = LowParse.Math
+
+let decode_int32le
+  (b: bytes { Seq.length b == 4 } )
+: Tot (v: U32.t { 0 <= U32.v v /\ U32.v v < 4294967296 } )
+= lemma_le_to_n_is_bounded b;
+  M.pow2_le_compat 32 32;
+  let res = le_to_n b in
+  assert (0 <= res /\ res < 4294967296);
+  U32.uint_to_t res
+
+let decode_int32le_injective
+  (b1 : bytes { Seq.length b1 == 4 } )
+  (b2 : bytes { Seq.length b2 == 4 } )
+: Lemma (decode_int32le b1 == decode_int32le b2
+        ==>
+        b1 == b2)
+= if (decode_int32le b1) = (decode_int32le b2) then
+  begin
+    lemma_le_to_n_is_bounded b1;
+    lemma_le_to_n_is_bounded b2;
+    assert (U32.v (U32.uint_to_t (le_to_n b1)) == le_to_n b1);
+    assert (U32.v (U32.uint_to_t (le_to_n b2)) == le_to_n b2);
+    assert (le_to_n b1 == le_to_n b2);
+    le_to_n_inj b1 b2
+  end
+  else
+    ()
+
+let decode_int32le_total_constant () : Lemma (make_total_constant_size_parser_precond 4 U32.t decode_int32le)
+= Classical.forall_intro_2 decode_int32le_injective
+  
+let parse_int32le : parser (total_constant_size_parser_kind 4) U32.t
+= decode_int32le_total_constant () ;
+  make_total_constant_size_parser 4 U32.t decode_int32le
+
+let serialize_int32le : serializer parse_int32le
+= fun (x : U32.t) -> n_to_le 4 (U32.v x)
+
+(* lemmas for inplace comparison in validators *)
+
+let le_to_n_0_eq
+  (b : bytes { Seq.length b == 0 } )
+: Lemma (le_to_n b == 0)
+= reveal_le_to_n b
+
+let le_to_n_1_eq
+  (b : bytes { Seq.length b == 1 } )
+: Lemma (le_to_n b == 
+    U8.v (Seq.index b 0))
+= assert_norm (pow2 8 == 256);
+  reveal_le_to_n b;
+  le_to_n_0_eq (Seq.tail b)
+
+let le_to_n_2_eq
+  (b : bytes { Seq.length b == 2 } )
+: Lemma (le_to_n b == 
+    U8.v (Seq.index b 0) + 
+    256 `FStar.Mul.op_Star` (U8.v (Seq.index b 1)))
+= assert_norm (pow2 8 == 256);
+  reveal_le_to_n b;
+  le_to_n_1_eq (Seq.tail b)
+
+let le_to_n_3_eq
+  (b : bytes { Seq.length b == 3 } )
+: Lemma (le_to_n b == 
+    U8.v (Seq.index b 0) + 
+    256 `FStar.Mul.op_Star` (U8.v (Seq.index b 1) + 
+    256 `FStar.Mul.op_Star` (U8.v (Seq.index b 2))))
+= assert_norm (pow2 8 == 256);
+  reveal_le_to_n b;
+  le_to_n_2_eq (Seq.tail b)
+
+let le_to_n_4_eq
+  (b : bytes { Seq.length b == 4 } )
+: Lemma (le_to_n b == 
+    U8.v (Seq.index b 0) + 
+    256 `FStar.Mul.op_Star` (U8.v (Seq.index b 1) + 
+    256 `FStar.Mul.op_Star` (U8.v (Seq.index b 2) + 
+    256 `FStar.Mul.op_Star` (U8.v (Seq.index b 3)))))
+= assert_norm (pow2 8 == 256);
+  reveal_le_to_n b;
+  le_to_n_3_eq (Seq.tail b)
+
+let decode_int32le_eq
+  (b : bytes { Seq.length b == 4 } )
+: Lemma
+  (U32.v (decode_int32le b) ==
+    U8.v (Seq.index b 0) + 
+    256 `FStar.Mul.op_Star` (U8.v (Seq.index b 1) + 
+    256 `FStar.Mul.op_Star` (U8.v (Seq.index b 2) + 
+    256 `FStar.Mul.op_Star` (U8.v (Seq.index b 3)))))
+= lemma_le_to_n_is_bounded b;
+  assert (U32.v (decode_int32le b) == le_to_n b);
+  le_to_n_4_eq b
+
